Define cardinal and lemmas

Ordinal.v
@@ -37,362 +37,6 @@ Proof.
   i. eapply H. eauto.
 Qed.
 
-
-Module Cardinality.
-  Variant le (A B: Type): Prop :=
-  | le_intro
-      (f: A -> B)
-      (INJ: forall a0 a1 (EQ: f a0 = f a1), a0 = a1)
-  .
-  Hint Constructors le.
-
-  Global Program Instance le_PreOrder: PreOrder le.
-  Next Obligation.
-  Proof.
-    ii. eapply le_intro with (f:=id). i. ss.
-  Qed.
-  Next Obligation.
-  Proof.
-    ii. inv H. inv H0. eapply le_intro with (f := compose f0 f).
-    i. eapply INJ. eapply INJ0. auto.
-  Qed.
-
-  Variant oto (A B: Type): Prop :=
-  | oto_intro
-      (f: A -> B)
-      (INJ: forall a0 a1 (EQ: f a0 = f a1), a0 = a1)
-      (SURJ: forall b, exists a, f a = b)
-  .
-  Hint Constructors oto.
-
-  Variant bij (A B: Type): Prop :=
-  | bij_intro
-      (f: A -> B) (g: B -> A)
-      (FG: forall a, g (f a) = a)
-      (GF: forall b, f (g b) = b)
-  .
-  Hint Constructors bij.
-
-  Lemma bij_oto_equiv A B: bij A B <-> oto A B.
-  Proof.
-    split; i.
-    - inv H. eapply oto_intro with (f:=f).
-      + i. eapply f_equal with (f:=g) in EQ.
-        repeat rewrite FG in EQ.  auto.
-      + i. exists (g b). auto.
-    - inv H. eapply choice in SURJ. des.
-      eapply bij_intro with (f:=f) (g:=f0); auto.
-  Qed.
-
-  Global Program Instance bij_Equivalence: Equivalence bij.
-  Next Obligation.
-  Proof.
-    ii. eapply bij_intro with (f:=id) (g:=id); auto.
-  Qed.
-  Next Obligation.
-  Proof.
-    ii. inv H. eapply bij_intro with (f:=g) (g:=f); auto.
-  Qed.
-  Next Obligation.
-  Proof.
-    ii. inv H. inv H0. eapply bij_intro with (f:=compose f0 f) (g:=compose g g0); auto.
-    - i. unfold compose. rewrite FG0. eapply FG.
-    - i. unfold compose. rewrite GF. eapply GF0.
-  Qed.
-
-  Global Program Instance oto_Equivalence: Equivalence oto.
-  Next Obligation.
-  Proof.
-    ii. eapply bij_oto_equiv. reflexivity.
-  Qed.
-  Next Obligation.
-  Proof.
-    ii. eapply bij_oto_equiv. eapply bij_oto_equiv in H. symmetry. auto.
-  Qed.
-  Next Obligation.
-  Proof.
-    ii. eapply bij_oto_equiv. eapply bij_oto_equiv in H. eapply bij_oto_equiv in H0.
-    transitivity y; auto.
-  Qed.
-
-  Lemma oto_le A B (OTO: oto A B): le A B.
-  Proof.
-    inv OTO. eapply le_intro with (f:=f). auto.
-  Qed.
-
-  Lemma bij_le A B (BIJ: bij A B): le A B.
-  Proof.
-    eapply bij_oto_equiv in BIJ. eapply oto_le; auto.
-  Qed.
-
-  Definition eq (A B: Type): Prop := le A B /\ le B A.
-
-  Lemma eq_le A B (EQ: eq A B): le A B.
-  Proof.
-    eapply EQ.
-  Qed.
-
-  Global Program Instance eq_Equivalence: Equivalence eq.
-  Next Obligation.
-  Proof.
-    ii. split; reflexivity.
-  Qed.
-  Next Obligation.
-  Proof.
-    ii. destruct H. split; auto.
-  Qed.
-  Next Obligation.
-  Proof.
-    ii. destruct H, H0. split; etransitivity; eauto.
-  Qed.
-
-  Global Program Instance le_eq_PartialOrder: PartialOrder eq le.
-  Next Obligation.
-  Proof. ss. Qed.
-
-  Section SANDWICH.
-    Variable A1 B A: Type.
-    Variable sub0: A1 -> B.
-    Variable sub1: B -> A.
-    Variable f: A -> A1.
-
-    Hypothesis SUB0: forall a0 a1 (EQ: sub0 a0 = sub0 a1), a0 = a1.
-    Hypothesis SUB1: forall b0 b1 (EQ: sub1 b0 = sub1 b1), b0 = b1.
-    Hypothesis INJ: forall a0 a1 (EQ: f a0 = f a1), a0 = a1.
-
-    Let Fixpoint aseq (n: nat) (a: A): A :=
-      match n with
-      | 0 => a
-      | S n' => sub1 (sub0 (f (aseq n' a)))
-      end.
-
-    Let Fixpoint bseq (n: nat) (b: B): A :=
-      match n with
-      | 0 => sub1 b
-      | S n' => sub1 (sub0 (f (bseq n' b)))
-      end.
-
-    Let bseq_aseq n:
-      forall b, exists a, bseq n b = aseq n a.
-    Proof.
-      induction n; ss.
-      - i. eauto.
-      - i. specialize (IHn b). des. exists a. rewrite IHn. auto.
-    Qed.
-
-    Let aseq_S_bseq n:
-      forall a, exists b, aseq (S n) a = bseq n b.
-    Proof.
-      induction n; ss.
-      - i. eauto.
-      - i. specialize (IHn a). des. exists b. rewrite IHn. auto.
-    Qed.
-
-    Let aseq_decrease n:
-      forall a0, exists a1, aseq (S n) a0 = aseq n a1.
-    Proof.
-      i. hexploit (aseq_S_bseq n a0). i. des.
-      hexploit (bseq_aseq n b). i. des.
-      exists a. rewrite H. auto.
-    Qed.
-
-    Let bseq_decrease n:
-      forall b0, exists b1, bseq (S n) b0 = bseq n b1.
-    Proof.
-      i. hexploit (bseq_aseq (S n) b0). i. des.
-      hexploit (aseq_S_bseq n a). i. des.
-      exists b. rewrite H. auto.
-    Qed.
-
-    Let in_gap (n: nat) (a1: A): Prop :=
-      (exists a0, aseq n a0 = a1) /\
-      (forall b0, bseq n b0 <> a1).
-
-    Let in_gap_step (n: nat) (a1: A):
-      in_gap (S n) a1 <->
-      (exists a0, in_gap n a0 /\ a1 = sub1 (sub0 (f a0))).
-    Proof.
-      unfold in_gap. split; i.
-      - des. ss. exists (aseq n a0). esplits; eauto.
-        ii. eapply (H0 b0). rewrite H1. auto.
-      - des. subst. ss. esplits; eauto. ii.
-        eapply SUB1 in H. eapply SUB0 in H.
-        eapply INJ in H. eapply H1; eauto.
-    Qed.
-
-    Let in_gap_all (a1: A): Prop :=
-      exists n, in_gap n a1.
-
-    Let is_g (g: A -> B): Prop :=
-      forall a,
-        (forall (GAP: in_gap_all a), g a = sub0 (f a)) /\
-        (forall (NGAP: ~ in_gap_all a), sub1 (g a) = a)
-    .
-
-    Let is_g_exists: exists g, is_g g.
-    Proof.
-      eapply (choice (fun a b =>
-                        (forall (GAP: in_gap_all a), b = sub0 (f a)) /\
-                        (forall (NGAP: ~ in_gap_all a), sub1 b = a))).
-      intros a. destruct (classic (in_gap_all a)).
-      - exists (sub0 (f a)). split; eauto. ss.
-      - destruct (classic (exists b, sub1 b = a)).
-        { des. exists b. splits; ss. }
-        exfalso. eapply H. exists 0. econs; ss; eauto.
-    Qed.
-
-    Let g_inj (g: A -> B) (G: is_g g):
-      forall a0 a1 (EQ: g a0 = g a1), a0 = a1.
-    Proof.
-      i. edestruct (G a0). edestruct (G a1).
-      destruct (classic (in_gap_all a0)), (classic (in_gap_all a1)).
-      - eapply H in H3. eapply H1 in H4.
-        rewrite H3 in *. rewrite H4 in *.
-        eapply SUB0 in EQ. eapply INJ in EQ; auto.
-      - exfalso. dup H3. dup H4.
-        eapply H in H5. eapply H2 in H6.
-        inv H3. eapply H4. exists (S x).
-        eapply in_gap_step. esplits; eauto.
-        rewrite <- H6. rewrite <- EQ. rewrite H5. auto.
-      - exfalso. dup H3. dup H4.
-        eapply H0 in H5. eapply H1 in H6.
-        inv H4. eapply H3. exists (S x).
-        eapply in_gap_step. esplits; eauto.
-        rewrite <- H6. rewrite <- EQ. rewrite H5. auto.
-      - eapply H0 in H3. eapply H2 in H4.
-        rewrite EQ in H3. rewrite H3 in *. auto.
-    Qed.
-
-    Let g_surj (g: A -> B) (G: is_g g):
-      forall b, exists a, g a = b.
-    Proof.
-      i. destruct (classic (in_gap_all (sub1 b))).
-      - dup H. eapply G in H0. inv H. destruct x.
-        { unfold in_gap in H1. des. ss. subst. exfalso. eapply H2; eauto. }
-        eapply in_gap_step in H1. des. eapply SUB1 in H2. subst.
-        dup H1. destruct (G a0). exploit H.
-        { exists x. auto. } i. eauto.
-      - dup H. eapply G in H0. eapply SUB1 in H0. eauto.
-    Qed.
-
-    Lemma sandwich_oto: oto A B.
-    Proof.
-      hexploit is_g_exists. i. des.
-      eapply oto_intro with (f:=g).
-      - eapply g_inj. auto.
-      - eapply g_surj. auto.
-    Qed.
-
-  End SANDWICH.
-
-  Lemma eq_oto_equiv A B: eq A B <-> oto A B.
-  Proof.
-    split; i.
-    - inv H. inv H0. inv H1.
-      eapply sandwich_oto with (A1:=A) (sub0:=f) (sub1:=f0) (f:=id); auto.
-    - eapply bij_oto_equiv in H. inv H. split.
-      + eapply le_intro with (f:=f).
-        i. eapply f_equal with (f:=g) in EQ. repeat rewrite FG in EQ. auto.
-      + eapply le_intro with (f:=g).
-        i. eapply f_equal with (f:=f) in EQ. repeat rewrite GF in EQ. auto.
-  Qed.
-
-  Lemma eq_bij_equiv A B: eq A B <-> bij A B.
-  Proof.
-    erewrite bij_oto_equiv. eapply eq_oto_equiv.
-  Qed.
-
-  Global Program Instance le_bij_PartialOrder: PartialOrder bij le.
-  Next Obligation.
-  Proof.
-    ii. ss. rewrite <- eq_bij_equiv. eauto.
-  Qed.
-
-  Global Program Instance le_oto_PartialOrder: PartialOrder oto le.
-  Next Obligation.
-  Proof.
-    ii. ss. rewrite <- eq_oto_equiv. eauto.
-  Qed.
-
-  Definition lt A B: Prop := le A B /\ ~ eq A B.
-
-  Lemma lt_le A B (LT: lt A B): le A B.
-  Proof.
-    eapply LT.
-  Qed.
-
-  Lemma lt_le_lt B A C (LT: lt A B) (LE: le B C): lt A C.
-  Proof.
-    inv LT. split.
-    - transitivity B; eauto.
-    - ii. inv H1. eapply H0. split; auto. transitivity C; auto.
-  Qed.
-
-  Lemma le_lt_lt B A C (LE: le A B) (LT: lt B C): lt A C.
-  Proof.
-    inv LT. split.
-    - transitivity B; eauto.
-    - ii. inv H1. eapply H0. split; auto. transitivity A; auto.
-  Qed.
-
-  Program Instance lt_StrictOrder: StrictOrder lt.
-  Next Obligation.
-  Proof.
-    ii. inv H. eapply H1. reflexivity.
-  Qed.
-  Next Obligation.
-  Proof.
-    ii. eapply (@lt_le_lt y); eauto. eapply lt_le; eauto.
-  Qed.
-
-  Lemma lt_not_le o0 o1 (LT: lt o0 o1) (LE: le o1 o0): False.
-  Proof.
-    eapply lt_StrictOrder. eapply le_lt_lt; eauto.
-  Qed.
-
-  Lemma lt_eq_lt A B0 B1 (EQ: eq B0 B1):
-    lt A B0 <-> lt A B1.
-  Proof.
-    split; i.
-    - inv EQ. eapply lt_le_lt; eauto.
-    - inv EQ. eapply lt_le_lt; eauto.
-  Qed.
-
-  Lemma eq_lt_lt A0 A1 B (EQ: eq A0 A1):
-    lt A0 B <-> lt A1 B.
-  Proof.
-    split; i.
-    - inv EQ. eapply le_lt_lt; eauto.
-    - inv EQ. eapply le_lt_lt; eauto.
-  Qed.
-
-  Lemma le_eq_le A B0 B1 (EQ: eq B0 B1):
-    le A B0 <-> le A B1.
-  Proof.
-    split; i.
-    - inv EQ. transitivity B0; auto.
-    - inv EQ. transitivity B1; auto.
-  Qed.
-
-  Lemma eq_le_le A0 A1 B (EQ: eq A0 A1):
-    le A0 B <-> le A1 B.
-  Proof.
-    split; i.
-    - inv EQ. transitivity A0; auto.
-    - inv EQ. transitivity A1; auto.
-  Qed.
-
-  Lemma le_eq_or_lt A B:
-    le A B <-> (lt A B \/ eq A B).
-  Proof.
-    split; i.
-    - destruct (classic (eq A B)); auto. left. split; auto.
-    - des.
-      + eapply H.
-      + eapply eq_le. auto.
-  Qed.
-End Cardinality.
-
 Module Ordinal.
   Section TYPE.
   Let MyT := Type.
@@ -1797,7 +1441,7 @@ Module Ordinal.
     Qed.
   End WO.
 
-  Theorem well_ordering_theorem (X: Type)
+  Lemma _well_ordering_theorem (X: Type)
     :
       exists (R: X -> X -> Prop),
         well_founded R /\
@@ -2017,7 +1661,7 @@ Module Ordinal.
       forall (c: B -> Prop) (CHAIN: forall b0 b1 (IN0: c b0) (IN1: c b1), R b0 b1 \/ b0 = b1 \/ R b1 b0),
       exists b_u, forall b (IN: c b), R b b_u \/ b = b_u.
 
-    Theorem zorn_lemma_lt:
+    Lemma _zorn_lemma_lt:
       exists b_m, forall b, ~ R b_m b.
     Proof.
       eapply NNPP. ii.
@@ -2048,10 +1692,10 @@ Module Ordinal.
       forall (c: B -> Prop) (CHAIN: forall b0 b1 (IN0: c b0) (IN1: c b1), R b0 b1 \/ R b1 b0),
       exists b_u, forall b (IN: c b), R b b_u.
 
-    Theorem zorn_lemma_antisym:
+    Lemma _zorn_lemma_antisym:
       exists b_m, forall b (LE: R b_m b), b = b_m.
     Proof.
-      hexploit (@zorn_lemma_lt B (fun b0 b1 => R b0 b1 /\ b0 <> b1)).
+      hexploit (@_zorn_lemma_lt B (fun b0 b1 => R b0 b1 /\ b0 <> b1)).
       { i. des. exploit antisym; eauto. }
       { i. des. splits; auto.
         - etransitivity; eauto.
@@ -2178,10 +1822,10 @@ Module Ordinal.
         eapply to_equiv_class_preserve; eauto. }
     Qed.
 
-    Theorem zorn_lemma:
+    Lemma _zorn_lemma:
       exists b_m, forall b (LE: R b_m b), R b b_m.
     Proof.
-      hexploit (@zorn_lemma_antisym _ equiv_class_rel); eauto. i. des.
+      hexploit (@_zorn_lemma_antisym _ equiv_class_rel); eauto. i. des.
       hexploit (proj2_sig b_m); eauto. i. des. exists a. i.
       eapply to_equiv_class_preserve in LE.
       eapply to_equiv_class_eq in H0; eauto. subst. ss.
@@ -2201,10 +1845,10 @@ Module Ordinal.
              (CHAIN: forall b0 b1 (IN0: c b0) (IN1: c b1), R b0 b1 \/ R b1 b0),
       exists b_u, forall b (IN: c b), R b b_u.
 
-    Theorem zorn_lemma_weak:
+    Lemma _zorn_lemma_weak:
       exists b_m, forall b (LE: R b_m b), R b b_m.
     Proof.
-      eapply zorn_lemma; eauto. i. destruct (classic (exists b, c b)).
+      eapply _zorn_lemma; eauto. i. destruct (classic (exists b, c b)).
       { eapply upperbound_exists; eauto. }
       { dup INHABITED. inv INHABITED. exists X. i. exfalso. eapply H; eauto. }
     Qed.
@@ -2273,7 +1917,7 @@ Module Ordinal.
       (forall a0 a1 (LT: R0 a0 a1), R1 a0 a1) /\
       (forall a0 a1, R1 a0 a1 \/ a0 = a1 \/ R1 a1 a0).
   Proof.
-    hexploit (well_ordering_theorem A); eauto. i. des.
+    hexploit (_well_ordering_theorem A); eauto. i. des.
     exists (extended R WF). splits.
     - eapply extended_well_founded; eauto.
     - eapply extended_incl; eauto.
@@ -2313,6 +1957,26 @@ Module Ordinal.
     destruct (total_le (from_wf_set WFA) (from_wf_set WFB)).
     - left. eapply from_wf_set_embed; eauto.
     - right. eapply from_wf_set_embed; eauto.
+  Qed.
+
+  Lemma set_comparable A B
+    :
+      (exists (f: A -> B), forall a0 a1 (EQ: f a0 = f a1), a0 = a1) \/
+      (exists (f: B -> A), forall b0 b1 (EQ: f b0 = f b1), b0 = b1).
+  Proof.
+    hexploit (@_well_ordering_theorem A); eauto. i. des.
+    hexploit (@_well_ordering_theorem B); eauto. i. des.
+    hexploit (from_wf_set_comparable H H1); eauto. i. des.
+    - left. exists f. i. destruct (H0 a0 a1) as [|[]]; auto.
+      + eapply H3 in H4. rewrite EQ in *. exfalso.
+        eapply (well_founded_irreflexive H1); eauto.
+      + eapply H3 in H4. rewrite EQ in *. exfalso.
+        eapply (well_founded_irreflexive H1); eauto.
+    - right. exists f. i. destruct (H2 b0 b1) as [|[]]; auto.
+      + eapply H3 in H4. rewrite EQ in *. exfalso.
+        eapply (well_founded_irreflexive H); eauto.
+      + eapply H3 in H4. rewrite EQ in *. exfalso.
+        eapply (well_founded_irreflexive H); eauto.
   Qed.
 
   Lemma from_wf_inj A B (RA: A -> A -> Prop) (RB: B -> B -> Prop)
@@ -2864,168 +2528,279 @@ Module Ordinal.
     eapply equiv_class_total.
   Qed.
 
-  Lemma cardinal_total_le A B: Cardinality.le A B \/ Cardinality.le B A.
-  Proof.
-  Admitted.
+  Section CARDINALITY.
+    Variant _cardinal_le (A B: Type): Prop :=
+    | _cardinal_le_intro
+        (f: A -> B)
+        (INJ: forall a0 a1 (EQ: f a0 = f a1), a0 = a1)
+    .
 
-  Section CARDINAL.
-    Variable A: MyT.
+    Let _cardinal_eq (A B: Type): Prop := _cardinal_le A B /\ _cardinal_le B A.
+    Let _cardinal_lt (A B: Type): Prop := _cardinal_le A B /\ ~ _cardinal_eq A B.
 
-    Definition is_cardinal (c: t): Prop :=
-      is_meet (fun o =>
-                 exists (R: A -> A -> Prop) (WF: well_founded R),
-                   (forall a0 a1, R a0 a1 \/ a0 = a1 \/ R a1 a0) /\
-                   eq (from_wf_set WF) o) c.
-
-    Lemma is_cardinal_exists: exists c, is_cardinal c.
+    Let _cardinal_total_le: forall (A B: Type), _cardinal_le A B \/ _cardinal_le B A.
     Proof.
-      eapply meet_exists.
-      hexploit (@well_ordering_theorem A); eauto. i. des.
-      exists (from_wf_set H), R, H. splits; auto. reflexivity.
+      i. hexploit (set_comparable A B). i. des.
+      - left. econs; eauto.
+      - right. econs; eauto.
     Qed.
 
-    Definition X: MyT :=
-      @sig
-        (@sigT (A -> Prop) (fun s => sig s -> sig s-> Prop))
-        (fun PR =>
-           well_founded (projT2 PR) /\
-           (forall a0 a1, projT2 PR a0 a1 \/ a0 = a1 \/ projT2 PR a1 a0) /\
-           (forall (f: A -> sig (projT1 PR)),
-               exists a0 a1, f a0 = f a1 /\ a0 <> a1)).
+    Section CARDINAL.
+      Variable A: MyT.
 
-    Definition Y (x: X): t :=
-      @from_wf_set (sig (projT1 (proj1_sig x))) _ (proj1 (proj2_sig x)).
+      Definition is_cardinal (c: t): Prop :=
+        is_meet (fun o =>
+                   exists (R: A -> A -> Prop) (WF: well_founded R),
+                     (forall a0 a1, R a0 a1 \/ a0 = a1 \/ R a1 a0) /\
+                     eq (from_wf_set WF) o) c.
 
-    Definition cardinal := @build X Y.
+      Lemma is_cardinal_exists: exists c, is_cardinal c.
+      Proof.
+        eapply meet_exists.
+        hexploit (@_well_ordering_theorem A); eauto. i. des.
+        exists (from_wf_set H), R, H. splits; auto. reflexivity.
+      Qed.
 
-    Lemma cardinal_lowerbound (R: A -> A -> Prop) (WF: well_founded R)
-          (TOTAL: forall a0 a1, R a0 a1 \/ a0 = a1 \/ R a1 a0):
-      le cardinal (from_wf_set WF).
-    Proof.
-      eapply build_spec. i. unfold Y.
-      destruct a as [[P0 R0] [WF0 [TOTAL0 SMALL]]]; ss.
-      replace (proj1 (conj WF0 (conj TOTAL0 SMALL))) with WF0.
-      2: { eapply well_founded_prop. }
-      destruct (total (from_wf_set WF) (from_wf_set WF0)); auto.
-      exfalso. exploit from_wf_set_embed; eauto. i. des.
-      hexploit (SMALL f); eauto. i. des.
-      destruct (TOTAL a0 a1) as [|[]]; ss.
-      { eapply x0 in H2. rewrite H0 in *.
-        eapply well_founded_irreflexive in H2; eauto. }
-      { eapply x0 in H2. rewrite H0 in *.
-        eapply well_founded_irreflexive in H2; eauto. }
-    Qed.
+      Lemma cardinal_unique c0 c1 (CARD0: is_cardinal c0) (CARD1: is_cardinal c1):
+        eq c0 c1.
+      Proof.
+        unfold is_cardinal, is_meet in *. des. split.
+        - eapply CARD4; eauto.
+        - eapply CARD2; eauto.
+      Qed.
 
-    Lemma cardinal_upperbound B (CARD: Cardinality.lt B A)
-          (R: B -> B -> Prop) (WF: well_founded R)
-      :
-        lt (from_wf_set WF) cardinal.
-    Proof.
-      inv CARD.
-      assert (CLT: ~ Cardinality.le A B).
-      { ii. eapply H0. econs; eauto. } inv H.
-      hexploit (from_wf_set_projected_rel_sig_eq WF _ INJ). i.
-      hexploit (well_order_extendable (projected_rel_sig_well_founded WF f INJ)). i. des.
-      hexploit (from_wf_set_le H2 (projected_rel_sig_well_founded WF f INJ) H1). i.
-      eapply le_lt_lt.
-      { etransitivity.
-        { eapply H. }
-        { eapply H4. }
-      }
-      assert ((fun (PR:(@sigT (A -> Prop) (fun s => sig s -> sig s-> Prop))) =>
-                 well_founded (projT2 PR) /\
-                 (forall a0 a1, projT2 PR a0 a1 \/ a0 = a1 \/ projT2 PR a1 a0) /\
-                 (forall (f: A -> sig (projT1 PR)),
-                     exists a0 a1, f a0 = f a1 /\ a0 <> a1)) (existT _ _ R1)).
-      { ss. splits; auto. i. eapply NNPP. ii. eapply CLT.
-        hexploit (choice (fun (a: A) (b: B) => proj1_sig (f0 a) = f b)).
-        { i.  hexploit (proj2_sig (f0 x)). i. des. eauto. }
-        i. des. eapply Cardinality.le_intro with (f:=f1). i.
-        eapply NNPP. ii. eapply f_equal with (f:=f) in EQ.
-        rewrite <- H6 in EQ. rewrite <- H6 in EQ.
-        eapply H5; eauto. exists a0, a1. splits; auto.
-        destruct (f0 a0), (f0 a1); auto. ss. subst. f_equal. eapply proof_irrelevance.
-      }
-      hexploit (@build_upperbound
-                  X Y
-                  (@exist
-                     (@sigT (A -> Prop) (fun s => sig s -> sig s-> Prop))
-                     (fun PR =>
-                        well_founded (projT2 PR) /\
-                        (forall a0 a1, projT2 PR a0 a1 \/ a0 = a1 \/ projT2 PR a1 a0) /\
-                        (forall (f: A -> sig (projT1 PR)),
-                            exists a0 a1, f a0 = f a1 /\ a0 <> a1))
-                     (@existT (A -> Prop) (fun s => sig s -> sig s-> Prop) _ R1)
-                     H5)).
-      ss. unfold Y. ss. i.
-      replace H1 with (proj1 H5); auto.
-    Qed.
+      Let X: MyT :=
+        @sig
+          (@sigT (A -> Prop) (fun s => sig s -> sig s-> Prop))
+          (fun PR =>
+             well_founded (projT2 PR) /\
+             (forall a0 a1, projT2 PR a0 a1 \/ a0 = a1 \/ projT2 PR a1 a0) /\
+             (forall (f: A -> sig (projT1 PR)),
+                 exists a0 a1, f a0 = f a1 /\ a0 <> a1)).
 
-    Lemma cardinal_supremum c
-          (UPPER: forall (B: MyT) (CARD: Cardinality.lt B A)
-                         (R: B -> B -> Prop) (WF: well_founded R),
-              lt (from_wf_set WF) c)
-      :
-        le cardinal c.
-    Proof.
-      eapply build_spec. i.
-      destruct a as [[P0 R0] [WF0 [TOTAL SMALL]]]; ss. unfold Y. ss.
-      replace (proj1 (conj WF0 (conj TOTAL SMALL))) with WF0.
-      2: { eapply well_founded_prop. } eapply UPPER.
-      assert (NLE: ~ Cardinality.le A (sig P0)).
-      { ii. inv H. hexploit (SMALL f); eauto. i. des.
-        eapply INJ in H. ss. }
-      destruct (cardinal_total_le A (sig P0)); ss.
-      econs; auto. ii. eapply NLE. eapply H0.
-    Qed.
+      Let Y (x: X): t :=
+        @from_wf_set (sig (projT1 (proj1_sig x))) _ (proj1 (proj2_sig x)).
 
-    Lemma cardinal_is_cardinal: is_cardinal cardinal.
-    Proof.
-      split.
-      - hexploit is_cardinal_exists. i. des.
-        unfold is_cardinal, is_meet in H. des.
-        exists R, WF. splits; auto. split.
-        2: { eapply cardinal_lowerbound; auto. }
-        hexploit (to_total_exists cardinal); eauto. i. des.
-        hexploit (cardinal_total_le A A0). i.
-        destruct (classic (Cardinality.le A A0)).
-        { transitivity (from_wf_set WF0).
-          2: { eapply H2. }
-          transitivity c.
-          { eapply H1. }
-          inv H5.
-          hexploit (projected_rel_rev_well_founded WF0 f); auto. i.
-          hexploit (H0 (from_wf_set H5)).
-          { eexists _, H5. splits; auto.
-            - i. destruct (H3 (f a0) (f a1)) as [|[]]; auto.
-            - reflexivity. }
-          i. transitivity (from_wf_set H5); auto.
-          eapply from_wf_set_inj; eauto.
-        }
-        { assert (CLT: Cardinality.lt A0 A).
-          { des; ss. eapply Cardinality.le_eq_or_lt in H4. des; auto.
-            exfalso. eapply H5. eapply H4. }
-          hexploit (cardinal_upperbound CLT WF0). i.
-          exfalso. eapply lt_not_le.
-          { eapply H6. }
-          { eapply H2. }
-        }
-      - i. des. eapply build_spec. i. unfold Y.
-        destruct a as [[P0 R0] [WF0 [TOTAL SMALL]]]; ss.
-        replace (proj1 (conj WF0 (conj TOTAL SMALL))) with WF0.
+      Definition cardinal := @build X Y.
+
+      Lemma cardinal_lowerbound (R: A -> A -> Prop) (WF: well_founded R)
+            (TOTAL: forall a0 a1, R a0 a1 \/ a0 = a1 \/ R a1 a0):
+        le cardinal (from_wf_set WF).
+      Proof.
+        eapply build_spec. i. unfold Y.
+        destruct a as [[P0 R0] [WF0 [TOTAL0 SMALL]]]; ss.
+        replace (proj1 (conj WF0 (conj TOTAL0 SMALL))) with WF0.
         2: { eapply well_founded_prop. }
-        eapply lt_eq_lt.
-        { symmetry. eapply IN0. }
         destruct (total (from_wf_set WF) (from_wf_set WF0)); auto.
         exfalso. exploit from_wf_set_embed; eauto. i. des.
         hexploit (SMALL f); eauto. i. des.
-        destruct (IN a0 a1) as [|[]]; ss.
+        destruct (TOTAL a0 a1) as [|[]]; ss.
         { eapply x0 in H2. rewrite H0 in *.
           eapply well_founded_irreflexive in H2; eauto. }
         { eapply x0 in H2. rewrite H0 in *.
           eapply well_founded_irreflexive in H2; eauto. }
+      Qed.
+
+      Lemma _cardinal_upperbound B (CARD: _cardinal_lt B A)
+            (R: B -> B -> Prop) (WF: well_founded R)
+        :
+          lt (from_wf_set WF) cardinal.
+      Proof.
+        inv CARD.
+        assert (CLT: ~ _cardinal_le A B).
+        { ii. eapply H0. econs; eauto. } inv H.
+        hexploit (from_wf_set_projected_rel_sig_eq WF _ INJ). i.
+        hexploit (well_order_extendable (projected_rel_sig_well_founded WF f INJ)). i. des.
+        hexploit (from_wf_set_le H2 (projected_rel_sig_well_founded WF f INJ) H1). i.
+        eapply le_lt_lt.
+        { etransitivity.
+          { eapply H. }
+          { eapply H4. }
+        }
+        assert ((fun (PR:(@sigT (A -> Prop) (fun s => sig s -> sig s-> Prop))) =>
+                   well_founded (projT2 PR) /\
+                   (forall a0 a1, projT2 PR a0 a1 \/ a0 = a1 \/ projT2 PR a1 a0) /\
+                   (forall (f: A -> sig (projT1 PR)),
+                       exists a0 a1, f a0 = f a1 /\ a0 <> a1)) (existT _ _ R1)).
+        { ss. splits; auto. i. eapply NNPP. ii. eapply CLT.
+          hexploit (choice (fun (a: A) (b: B) => proj1_sig (f0 a) = f b)).
+          { i.  hexploit (proj2_sig (f0 x)). i. des. eauto. }
+          i. des. eapply _cardinal_le_intro with (f:=f1). i.
+          eapply NNPP. ii. eapply f_equal with (f:=f) in EQ.
+          rewrite <- H6 in EQ. rewrite <- H6 in EQ.
+          eapply H5; eauto. exists a0, a1. splits; auto.
+          destruct (f0 a0), (f0 a1); auto. ss. subst. f_equal. eapply proof_irrelevance.
+        }
+        hexploit (@build_upperbound
+                    X Y
+                    (@exist
+                       (@sigT (A -> Prop) (fun s => sig s -> sig s-> Prop))
+                       (fun PR =>
+                          well_founded (projT2 PR) /\
+                          (forall a0 a1, projT2 PR a0 a1 \/ a0 = a1 \/ projT2 PR a1 a0) /\
+                          (forall (f: A -> sig (projT1 PR)),
+                              exists a0 a1, f a0 = f a1 /\ a0 <> a1))
+                       (@existT (A -> Prop) (fun s => sig s -> sig s-> Prop) _ R1)
+                       H5)).
+        ss. unfold Y. ss. i.
+        replace H1 with (proj1 H5); auto.
+      Qed.
+
+      Lemma _cardinal_supremum c
+            (UPPER: forall (B: MyT) (CARD: _cardinal_lt B A)
+                           (R: B -> B -> Prop) (WF: well_founded R),
+                lt (from_wf_set WF) c)
+        :
+          le cardinal c.
+      Proof.
+        eapply build_spec. i.
+        destruct a as [[P0 R0] [WF0 [TOTAL SMALL]]]; ss. unfold Y. ss.
+        replace (proj1 (conj WF0 (conj TOTAL SMALL))) with WF0.
+        2: { eapply well_founded_prop. } eapply UPPER.
+        assert (NLE: ~ _cardinal_le A (sig P0)).
+        { ii. inv H. hexploit (SMALL f); eauto. i. des.
+          eapply INJ in H. ss. }
+        destruct (_cardinal_total_le A (sig P0)); ss.
+        econs; auto. ii. eapply NLE. eapply H0.
+      Qed.
+
+      Lemma cardinal_is_cardinal: is_cardinal cardinal.
+      Proof.
+        split.
+        - hexploit is_cardinal_exists. i. des.
+          unfold is_cardinal, is_meet in H. des.
+          exists R, WF. splits; auto. split.
+          2: { eapply cardinal_lowerbound; auto. }
+          hexploit (to_total_exists cardinal); eauto. i. des.
+          hexploit (_cardinal_total_le A A0). i.
+          destruct (classic (_cardinal_le A A0)).
+          { transitivity (from_wf_set WF0).
+            2: { eapply H2. }
+            transitivity c.
+            { eapply H1. }
+            inv H5.
+            hexploit (projected_rel_rev_well_founded WF0 f); auto. i.
+            hexploit (H0 (from_wf_set H5)).
+            { eexists _, H5. splits; auto.
+              - i. destruct (H3 (f a0) (f a1)) as [|[]]; auto.
+              - reflexivity. }
+            i. transitivity (from_wf_set H5); auto.
+            eapply from_wf_set_inj; eauto.
+          }
+          { assert (CLT: _cardinal_lt A0 A).
+            { des; ss. econs; eauto. ii. inv H6. ss. }
+            hexploit (_cardinal_upperbound CLT WF0). i.
+            exfalso. eapply lt_not_le.
+            { eapply H6. }
+            { eapply H2. }
+          }
+        - i. des. eapply build_spec. i. unfold Y.
+          destruct a as [[P0 R0] [WF0 [TOTAL SMALL]]]; ss.
+          replace (proj1 (conj WF0 (conj TOTAL SMALL))) with WF0.
+          2: { eapply well_founded_prop. }
+          eapply lt_eq_lt.
+          { symmetry. eapply IN0. }
+          destruct (total (from_wf_set WF) (from_wf_set WF0)); auto.
+          exfalso. exploit from_wf_set_embed; eauto. i. des.
+          hexploit (SMALL f); eauto. i. des.
+          destruct (IN a0 a1) as [|[]]; ss.
+          { eapply x0 in H2. rewrite H0 in *.
+            eapply well_founded_irreflexive in H2; eauto. }
+          { eapply x0 in H2. rewrite H0 in *.
+            eapply well_founded_irreflexive in H2; eauto. }
+      Qed.
+    End CARDINAL.
+
+    Lemma _cardinal_le_iff A B:
+      _cardinal_le A B <-> le (cardinal A) (cardinal B).
+    Proof.
+      split. i.
+      - hexploit (cardinal_is_cardinal B). i. destruct H0. des.
+        transitivity (from_wf_set WF); auto.
+        2: { eapply H2. }
+        inv H. transitivity (from_wf_set (projected_rel_rev_well_founded WF f INJ)).
+        { eapply cardinal_is_cardinal.
+          exists _, (projected_rel_rev_well_founded WF f INJ). splits; auto.
+          - i. destruct (H0 (f a0) (f a1)) as [|[]]; auto.
+          - reflexivity.
+        }
+        { eapply from_wf_set_inj. instantiate (1:=f). i. apply LT. }
+      - hexploit (cardinal_is_cardinal B). i. destruct H. des.
+        i. eapply NNPP. ii. destruct (_cardinal_total_le A B); ss.
+        hexploit (_cardinal_upperbound).
+        { split; eauto. ii. inv H5; ss. }
+        instantiate (1:=WF). i. eapply lt_not_le; eauto.
+        transitivity (cardinal B); auto. apply H2.
     Qed.
-  End CARDINAL.
+
+    Lemma _cardinal_eq_iff A B:
+      _cardinal_eq A B <-> eq (cardinal A) (cardinal B).
+    Proof.
+      split. i.
+      - split.
+        + eapply _cardinal_le_iff; auto. apply H.
+        + eapply _cardinal_le_iff; auto. apply H.
+      - split.
+        + eapply _cardinal_le_iff; auto. apply H.
+        + eapply _cardinal_le_iff; auto. apply H.
+    Qed.
+
+    Lemma _cardinal_lt_iff A B:
+      _cardinal_lt A B <-> lt (cardinal A) (cardinal B).
+    Proof.
+      split; i.
+      - inv H. eapply _cardinal_le_iff in H0.
+        eapply le_eq_or_lt in H0. des; auto.
+        exfalso. eapply H1. eapply _cardinal_eq_iff; eauto.
+      - split.
+        + eapply _cardinal_le_iff. eapply lt_le; eauto.
+        + ii. eapply _cardinal_eq_iff in H0.
+          eapply lt_not_le; eauto. eapply H0.
+    Qed.
+
+    Lemma cardinal_size_le A B (R: B -> B -> Prop) (WF: well_founded R)
+          (TOTAL: forall b0 b1, R b0 b1 \/ b0 = b1 \/ R b1 b0)
+          (LE: le (cardinal A) (from_wf_set WF)):
+      le (cardinal A) (cardinal B).
+    Proof.
+      hexploit (cardinal_is_cardinal A); auto. i. inv H. des.
+      hexploit (@from_wf_set_embed _ _ _ _ WF0 WF); auto.
+      { transitivity (cardinal A); auto. apply H2. }
+      i. des. eapply _cardinal_le_iff.
+      eapply _cardinal_le_intro with (f:=f). i.
+      destruct (H0 a0 a1) as [|[]]; auto.
+      - eapply H in H3. rewrite EQ in *.
+        exfalso. eapply (well_founded_irreflexive WF); eauto.
+      - eapply H in H3. rewrite EQ in *.
+        exfalso. eapply (well_founded_irreflexive WF); eauto.
+    Qed.
+
+    Lemma cardinal_size_eq A B (R: B -> B -> Prop) (WF: well_founded R)
+          (TOTAL: forall b0 b1, R b0 b1 \/ b0 = b1 \/ R b1 b0)
+          (EQ: eq (cardinal A) (from_wf_set WF)):
+      eq (cardinal A) (cardinal B).
+    Proof.
+      split; i.
+      - eapply cardinal_size_le; eauto. eapply EQ.
+      - transitivity (from_wf_set WF).
+        + eapply (cardinal_is_cardinal B). esplits; eauto. reflexivity.
+        + eapply EQ.
+    Qed.
+  End CARDINALITY.
+
+  Section ALEPH.
+    Section NEXT.
+      Variable A: MyT.
+      Let next_o := @build (
+
+    Let next_cardinal (A: MyT): MyT :=
+      build (fun
+
+    Let next (o: t):
+
+  Section INCACCESSIBLE.
+
+
 End TYPE.
 End Ordinal.
 
